

Math 574

class # 21

11/11/2025

## Convergence of Implicit - Euler - Galerkin Method

Theorem (21.1): Suppose the hypotheses of Theorem (20.2) are satisfied. Assume that  $u$  is a solution to

$$(21.1) \quad (\partial_t u, \psi) + (\nabla u, \nabla \psi) = (f, \psi),$$

for all  $\psi \in H_0^1(\Omega)$ , for all  $t \in (0, T]$ , where  $u(\cdot, 0) = v$ , and  $u$  has the regularities

$$u \in L^2(0, T; H_0^1 \cap H^{r+1})$$

$$\cap H^1(0, T; H^{r+1})$$

$$\cap H^2(0, T; L^2)$$

and

$$v \in H_0^1 \cap H^{r+1}$$

$$\Rightarrow \int_0^T \|\partial_{tt} u\|_{L^2}^2 dt < \infty$$

Suppose  $u_n^k \in V_n = \mathcal{H}_{0,r}$ ,  $k=0, \dots, K$ , satisfies

$$(21.2) \quad (\delta_s u_n^k, \psi) + (\nabla u_n^k, \nabla \psi) = (f, \psi)$$

for all  $\psi \in V_n$ , with

$$u_n^0 = v_n = P_n v \in V_n,$$

$$\delta_s u_n^k := \frac{u_n^k - u_n^{k-1}}{s},$$

$$\delta := \frac{T}{K}.$$

Suppose that

$$\|v - v_h\|_{L^2} \leq Ch^{r+1} \|v\|_{H^{r+1}}.$$

Then

$$(21.3) \quad \|u_h^k - u(t_k)\|_{L^2} \leq Ch^{r+1} \left( \|v\|_{H^{r+1}} + \int_0^{t_k} \|\partial_t u\|_{H^{r+1}} dz \right) + \delta \int_0^{t_k} \|\partial_t u\|_{L^2} dz.$$

Proof: As before, set

$$p(t) := u(t) - R_h u(t)$$

$$\theta^k := R_h u(t_k) - u_h^k \quad k=0, 1, \dots, K,$$

where

$$t_k = \delta \cdot k, \quad k=0, 1, \dots, K.$$

Then

$$\begin{aligned} u(t_k) - u_h^k &= p(t_k) + \theta^k \\ &= p^k + \theta^k, \end{aligned}$$

where

$$p^k := p(t_k).$$

Note that  $\theta^k$  is defined only at  $t_k$ , that is, at discrete times, whereas  $p$  is defined at all times.

As before

$$\|p(t_k)\|_{L^2} \leq C h^{r+1} \left( \|v\|_{H^{r+1}} + \int_0^{t_k} \|\partial_t u(x)\|_{H^{r+1}} dx \right),$$

for  $k=0, 1, \dots, K$ . By the defn of  $R_h$ ,

$$(\partial_t u, \psi) + (\nabla R_h u, \nabla \psi) = (f, \psi), \quad \forall \psi \in V_h.$$

For  $k=1, \dots, K$ , and for all  $\psi \in V_h$ ,

$$(21.4) \quad (R_h(\delta_s u(t_k)), \psi) + (\nabla R_h u(t_k), \nabla \psi) = (f(t_k), \psi) + (w^k, \psi)$$

where

$$\delta_s u(t) := \frac{u(t) - u(t-s)}{s}, \quad t \in [s, T],$$

and

$$w(t) := R_h(\delta_s u(t)) - \partial_t u(t), \quad w^k := w(t_k).$$

Subtracting (21.2) (the Backward Euler-Galerkin scheme) from (21.4) to get

$$(\delta_s \theta^k, \psi) + (\nabla \theta^k, \nabla \psi) = (w^k, \psi), \quad \forall \psi \in V_h.$$

Next, set  $\psi = \theta^k$ , to get

$$(\theta^k - \theta^{k-1}, \theta^k) + s |\theta^k|_{H^1}^2 = s (w^k, \theta^k)$$

Then

$$\begin{aligned} \|\theta^k\|_{L^2}^2 - (\theta^{k-1}, \theta^k) + s |\theta^k|_{H^1}^2 &= s (w^k, \theta^k) \\ &\stackrel{C.S.}{\leq} s \|w^k\|_{L^2} \|\theta^k\|_{L^2} \end{aligned}$$

$$(\theta^{k-1}, \theta^k) \leq \|\theta^{k-1}\|_{L^2} \|\theta^k\|_{L^2} \Rightarrow -\|\theta^{k-1}\|_{L^2} \|\theta^k\|_{L^2} \leq -(\theta^{k-1}, \theta^k)$$

This implies

$$\|\theta^k\|_{L^2}^2 - \|\theta^{k-1}\|_{L^2} \|\theta^k\|_{L^2} \leq s \|\omega^k\|_{L^2} \|\theta^k\|_{L^2},$$

which, in turn, implies

$$\|\theta^k\|_{L^2} - \|\theta^{k-1}\|_{L^2} \leq s \|\omega^k\|_{L^2}$$

for  $k=1, 2, \dots, K$ . Summing from  $k=1$  to  $k=l$

$$(21.5) \quad \|\theta^l\|_{L^2} \leq \|\theta^0\|_{L^2} + s \sum_{k=1}^l \|\omega^k\|_{L^2}$$

for any  $1 \leq l \leq K$ . Define

$$\omega_1^k := (R_h - I) \delta_s u(t_k),$$

$$\omega_2^k := \delta_s u(t_k) - \partial_t u(t_k).$$

Then

$$\omega^k = \omega_1^k + \omega_2^k.$$

It follows that

$$\begin{aligned} \omega_1^k &= \frac{1}{s} (R_h - I) \int_{t_{k-1}}^{t_k} \partial_t u(\tau) d\tau \\ &= \frac{1}{s} \int_{t_{k-1}}^{t_k} (R_h - I) \partial_t u(\tau) d\tau \end{aligned}$$

$$\begin{aligned} &\left\| \int_{t_a}^{t_b} u(\tau) d\tau \right\| \\ &\leq \int_{t_a}^{t_b} \|u(\tau)\| d\tau \end{aligned}$$

Then

$$\begin{aligned} \|\omega_1^k\|_{L^2} &\leq \frac{1}{s} \int_{t_{k-1}}^{t_k} \|R_h \partial_t u(\tau) - \partial_t u(\tau)\|_{L^2} d\tau \\ &\leq \frac{1}{s} C h^{r+1} \int_{t_{k-1}}^{t_k} \|\partial_t u(\tau)\|_{H^{r+1}} d\tau. \end{aligned}$$

Taylor's Theorem:

$$u(t_{k-1}) = u(t_k) + \partial_t u(t_k)(t_{k-1} - t_k) + \tilde{R}_2[u](t_k)$$

(21.6) So

$$S \sum_{k=1}^l \|w_1^k\|_{L^2} \leq C h^{r+1} \int_0^{t_l} \|\partial_t u(\tau)\|_{L^2} d\tau$$

To estimate  $w_2^k$ , note

$$\begin{aligned} S w_2^k &= u(t_k) - u(t_{k-1}) - S \partial_t u(t_k) \\ &= - \int_{t_{k-1}}^{t_k} (\tau - t_{k-1}) \partial_{tt} u(\tau) d\tau, \end{aligned}$$

where we have used Taylor's Theorem with integral remainder. (Remember that?)

Thus,

(21.7)

$$\begin{aligned} S \sum_{k=1}^l \|w_2^k\|_{L^2} &\leq \sum_{k=1}^l \int_{t_{k-1}}^{t_k} |\tau - t_{k-1}| \cdot \|\partial_{tt} u(\tau)\|_{L^2} d\tau \\ &\leq S \int_0^{t_l} \|\partial_{tt} u(\tau)\|_{L^2} d\tau. \end{aligned}$$

Also, observe

(21.8)

$$\begin{aligned} \|\theta^0\|_{L^2} &= \|R_h v - u_h^0\|_{L^2} \\ &\leq \|R_h v - v\|_{L^2} + \|v - v_h\|_{L^2} \\ &\leq C h^{r+1} \|v\|_{H^{r+1}} \end{aligned}$$

Combining (21.5) - (21.8)

$$\begin{aligned}
\|\theta^{\ell}\|_{L^2} &\leq \|\theta^0\|_{L^2} + s \sum_{k=1}^{\ell} \|w_1^k\|_{L^2} + s \sum_{k=1}^{\ell} \|w_2^k\|_{L^2} \\
&\leq C h^{r+1} \|v\|_{H^{r+1}} + C h^{r+1} \int_0^{t_{\ell}} \|\partial_t u(\tau)\|_{H^{r+1}} d\tau \\
&\quad + s \int_0^{t_{\ell}} \|\partial_{tt} u(\tau)\|_{L^2} d\tau
\end{aligned}$$

Since

$$\|\rho^{\ell}\|_{L^2} \leq C h^{r+1} \left( \|v\|_{H^{r+1}} + \int_0^{t_{\ell}} \|\partial_t u\|_{H^{r+1}} d\tau \right),$$

it follows that

$$\begin{aligned}
\|u(t_k) - u_h^k\|_{L^2} &\leq \|\theta^k\|_{L^2} + \|\rho^k\|_{L^2} \\
&\leq C h^{r+1} \left( \|v\|_{H^{r+1}} + \int_0^{t_k} \|\partial_t u(\tau)\|_{H^{r+1}} d\tau \right) \\
&\quad + s \int_0^{t_k} \|\partial_{tt} u(\tau)\|_{L^2} d\tau \quad ///
\end{aligned}$$

### Crank - Nicholson - Galerkin Method

Given  $u_h^{k-1} \in V_h \subset H_0^1(\Omega)$ , find  $u_h^k \in V_h$ , such that

$$(21.9) \quad \left( \frac{u_h^k - u_h^{k-1}}{s}, \psi \right) + \frac{1}{2} \left( \nabla(u_h^k + u_h^{k-1}), \nabla \psi \right) = (f(t_{k-1/2}), \psi)$$

for all  $\psi \in V_h$ , for  $k=1, 2, \dots, K = T/s$ ,

where

$$u_n^0 = v_n = P_h v \in V_h$$

Theorem (21.2): Suppose that either

$$\|v_n\|_{L^2}^2 \leq C + \|v\|_{L^2}^2$$

where  $C > 0$  is independent of  $h$  and  $s$ . Then

$$\max_{0 \leq k \leq K} \|u_n^k\|_{L^2}^2 \leq C$$

and

$$s \sum_{k=1}^K \left| \frac{1}{2} (u_n^k + u_n^{k-1}) \right|_{H^1}^2 \leq C$$

for some  $C > 0$  that is independent of  $s$  and  $h$ .

Proof: In (21.9), set

$$\psi = u_n^{k-1/2} := \frac{1}{2} (u_n^k + u_n^{k-1}) \in V_h$$

Then, for  $k=1, \dots, K$ ,

$$\frac{1}{2s} \|u_n^k\|_{L^2}^2 - \frac{1}{2s} \|u_n^{k-1}\|_{L^2}^2 + |u_n^{k-1/2}|_{H^1}^2$$

$$= (f(t_{k-1/2}), u_n^{k-1/2})$$

C.S.

$$\leq \|f(t_{k-1/2})\|_{L^2} \|u_n^{k-1/2}\|_{L^2}$$

Poincaré

$$\leq \|f(t_{k-1/2})\|_{L^2} C |u_n^{k-1/2}|_{H^1}$$

AGI

$$\leq \frac{C^2}{2} \|f(t_{k-1/2})\|_{L^2}^2 + \frac{1}{2} |u_n^{k-1/2}|_{H^1}^2$$

Thus,

$$\frac{1}{2s} \|u_n^k\|_{L^2}^2 - \frac{1}{2s} \|u_n^{k-1}\|_{L^2}^2 + \frac{1}{2} |u_n^{k-1/2}|_{\#}^2 \leq \frac{c^2}{2} \|f(t_{k-1/2})\|_{L^2}^2$$

which implies

$$\|u_n^k\|_{L^2}^2 - \|u_n^{k-1}\|_{L^2}^2 + s |u_n^{k-1/2}|_{\#}^2 \leq sc^2 \|f(t_{k-1/2})\|_{L^2}^2.$$

Summing from  $k=1$  to  $k=l$ ,  $1 \leq l \leq K$ , we get

$$\begin{aligned} \|u_n^l\|_{L^2}^2 + s \sum_{k=1}^l |u_n^{k-1/2}|_{\#}^2 &\leq \|v_n\|_{L^2}^2 \\ &\quad + sc^2 \sum_{k=1}^l \|f(t_{k-1/2})\|_{L^2}^2 \\ &\leq C + \|v\|_{L^2}^2 \\ &\quad + sc^2 \sum_{k=1}^K \|f(t_{k-1/2})\|_{L^2}^2 \\ &\leq C + \|v\|_{L^2}^2 \\ &\quad + C + c^2 \int_0^T \|f(t)\|_{L^2}^2 dt \\ &= C, \end{aligned}$$

and  $C > 0$  is independent of  $h$  and  $s$ . ///